Simplify liveness.

extraction/lvcc.ml
@@ -37,7 +37,7 @@ let main () =
       let file_chan = open_in !infile in
       let lexbuf = Lexing.from_channel  file_chan in
       let ilin = Parser.program Lexer.token lexbuf in
-      let _ =  Printf.printf "Input:\n%s\n\n" (* (print_nstmt !ids 0 ilin) *) "a"  in
+      let _ =  Printf.printf "Input:\n%s\n\n" (print_nstmt !ids 0 ilin) in
       let ili = (match Lvc.toDeBruijn ilin with
 		 | Lvc.Success ili -> ili
 		 | Lvc.Error e -> raise (Compiler_error "Converting to de bruijn failed (did you define all functions?)"))
@@ -66,10 +66,9 @@ let main () =
       in
       let res =
 	if !toILI then
-	  let _ = Printf.printf "\nbefore fromILF\n" in
           (match Lvc.fromILF parallel_move generic_first sopt with
 	   | Lvc.Success ili ->
-	      Printf.printf "\nto IL/I compilate:\n%s\n\nXXX\n\n\n" (* (print_stmt !ids 0 ili) *) "a";
+	      Printf.printf "\nto IL/I compilate:\n%s\n\n" (print_stmt !ids 0 ili);
 	      ili
 	   | Lvc.Error e -> raise (Compiler_error (implode e))
 	  )
