LivenessAnalysis.v
@@ -26,12 +26,17 @@ Definition liveness_transform (DL:list (set var * params)) st a :=
     | stmtLet x e s as st, anni1 d =>
       (d \ {{x}}) ∪ (if [x ∈ d] then Exp.freeVars e else ∅)
     | stmtIf e s t as st, anni2 ds dt =>
-      Exp.freeVars e ∪ ds ∪ dt
+      if [exp2bool e = Some true] then
+        ds
+      else if [ exp2bool e = Some false ] then
+        dt
+      else
+        Exp.freeVars e ∪ ds ∪ dt
     | stmtApp f Y as st, anni0 =>
       let (lv,Z) := nth (counted f) DL (∅,nil) in
       lv \ of_list Z ∪ list_union (List.map Exp.freeVars (filter_by (fun x => B[x ∈ lv]) Z Y))
     | stmtReturn e as st, anni0 => Exp.freeVars e
-    | stmtExtern x f Y s as st, anni1 d=>
+    | stmtExtern x f Y s as st, anni1 d =>
       (d \ {{x}}) ∪ list_union (List.map Exp.freeVars Y)
     | stmtFun Z s t as st, anni2 ds dt =>
        (ds \ of_list Z) ∪ dt
