TrueLiveness.v
@@ -1,0 +1,72 @@
+Require Import AllInRel List Map Env DecSolve.
+Require Import IL Annotation AutoIndTac Bisim Exp MoreExp Filter.
+Require Export Liveness.
+
+Set Implicit Arguments.
+
+Local Hint Resolve incl_empty minus_incl incl_right incl_left.
+
+
+Inductive true_live_sound (i:overapproximation)
+  : list (set var *params) -> stmt -> ann (set var) -> Prop :=
+| TLOpr x Lv b lv e al
+  :  true_live_sound i Lv b al
+  -> (x ∈ getAnn al -> live_exp_sound e lv)
+  -> (getAnn al\{{x}}) ⊆ lv
+  -> (x ∉ getAnn al -> lv ⊆ getAnn al \ {{x}})
+  -> true_live_sound i Lv (stmtLet x e b) (ann1 lv al)
+| TLIf Lv e b1 b2 lv al1 al2
+  :  true_live_sound i Lv b1 al1
+  -> true_live_sound i Lv b2 al2
+  -> (exp2bool e = None -> live_exp_sound e lv)
+  -> (exp2bool e <> Some false -> getAnn al1 ⊆ lv)
+  -> (exp2bool e = Some true -> lv ⊆ getAnn al1)
+  -> (exp2bool e <> Some true -> getAnn al2 ⊆ lv)
+  -> (exp2bool e = Some false -> lv ⊆ getAnn al2)
+  -> true_live_sound i Lv (stmtIf e b1 b2) (ann2 lv al1 al2)
+| TLGoto l Y Lv lv blv Z
+  : get Lv (counted l) (blv,Z)
+  -> (if isImperative i then  (blv \ of_list Z ⊆ lv) else True)
+  -> argsLive lv blv Y Z
+  -> length Y = length Z
+  -> true_live_sound i Lv (stmtApp l Y) (ann0 lv)
+| TLReturn Lv e lv
+  : live_exp_sound e lv
+  -> true_live_sound i Lv (stmtReturn e) (ann0 lv)
+| TLExtern x Lv b lv Y al f
+  : true_live_sound i Lv b al
+  -> (forall n y, get Y n y -> live_exp_sound y lv)
+  -> (getAnn al\{{x}}) ⊆ lv
+  -> x ∈ getAnn al
+  -> true_live_sound i Lv (stmtExtern x f Y b) (ann1 lv al)
+| TLLet Lv s Z b lv als alb
+  : true_live_sound i ((getAnn als,Z)::Lv) s als
+  -> true_live_sound i ((getAnn als,Z)::Lv) b alb
+  -> (if isFunctional i then (getAnn als \ of_list Z ⊆ lv) else True)
+  -> getAnn alb ⊆ lv
+  -> true_live_sound i Lv (stmtFun Z s b)(ann2 lv als alb).
+
+
+Lemma true_live_sound_overapproximation_I Lv s slv
+: true_live_sound FunctionalAndImperative Lv s slv -> true_live_sound Imperative Lv s slv.
+Proof.
+  intros. general induction H; simpl in * |- *; econstructor; simpl; eauto.
+Qed.
+
+Lemma true_live_sound_overapproximation_F Lv s slv
+: true_live_sound FunctionalAndImperative Lv s slv -> true_live_sound Functional Lv s slv.
+Proof.
+  intros. general induction H; simpl in * |- *; econstructor; simpl; eauto.
+Qed.
+
+Lemma true_live_sound_annotation i Lv s slv
+: true_live_sound i Lv s slv -> annotation s slv.
+Proof.
+  intros. general induction H; econstructor; eauto.
+Qed.
+
+(*
+*** Local Variables: ***
+*** coq-load-path: (("." "Lvc")) ***
+*** End: ***
+*)
